Samples/sample_mutex.lean
@@ -1,5 +1,6 @@
 import Mt.Reservation
 import Mt.Task
+import Mt.Thread
 
 namespace SampleMutex
 
@@ -29,7 +30,7 @@ def spec : Mt.Spec :={
 open Mt
 open Mt.TaskM
 
-def thread1 : TaskM spec Unit :=do
+def thread1 : Thread spec :=mk_thread do
   -- lock mutex
   atomic_blocking_rmr (λ ⟨_, locked⟩ => locked = false) λ (s : State) => ⟨⟨⟩, {s with locked :=true}⟩
   
@@ -40,7 +41,7 @@ def thread1 : TaskM spec Unit :=do
   -- release mutex
   atomic_read_modify λ s => {s with locked :=false}
 
-def thread2 : TaskM spec Unit :=do
+def thread2 : Thread spec :=mk_thread do
   -- lock mutex
   atomic_blocking_rmr (λ ⟨_, locked⟩ => locked = false) λ (s : State) => ⟨⟨⟩, {s with locked :=true}⟩
   
@@ -71,8 +72,18 @@ theorem validate.elim_locked {env_r : Reservation} {d s'} :
   . rfl
   constructor <;> rfl
 
-theorem thread1_valid : thread1.valid' Mt.Lock.Unlocked :=by
-  rw [valid']
+theorem valid_bind_mutex_lock {T : Type} {cont : TaskM spec T} {assuming motive}
+  (cont_valid : ∀ x : Nat, cont.valid
+    (Lock.Locked ⟨x, x⟩)
+    (λ _ => true)
+    (motive))
+  : TaskM.valid (spec :=spec) (T :=T)
+    (do
+      atomic_blocking_rmr
+        (λ ⟨_, locked⟩ => locked = false)
+        λ (s : State) => ⟨⟨⟩, {s with locked :=true}⟩
+      cont
+    ) Lock.Unlocked assuming motive :=by
   apply valid_bind (spec :=spec) λ ⟨⟩ r => r.is_locked_and_valid Data.valid
   . -- verify mutex lock
     apply valid_blocking_rmr
@@ -89,8 +100,34 @@ theorem thread1_valid : thread1.valid' Mt.Lock.Unlocked :=by
   intro r ⟨⟩ is_locked_and_valid
   cases r <;> try contradiction
   rename_i data0
-  let ⟨x0, y0⟩ :=data0 ; clear data0
+  let ⟨x0, _⟩ :=data0 ; clear data0
   cases is_locked_and_valid
+  exact cont_valid x0
+
+theorem valid_mutex_release {assuming data}
+  (data_valid : data.valid)
+  : TaskM.valid (spec :=spec) (T :=Unit)
+    (atomic_read_modify λ s => {s with locked :=false})
+    (Lock.Locked data)
+    assuming
+    (λ _ r => r = Lock.Unlocked) :=by
+  apply valid_rm
+  simp only [spec, Lock.add_unlocked]
+  intro env_r ⟨data', locked ⟩ _ initial_valid
+  exists Lock.Unlocked
+  have : data = data' :=initial_valid.elim_locked.right.left
+  
+  simp only [initial_valid.elim_locked, and_true]
+  
+  apply validate.unlocked
+  rw [<- this]
+  exact data_valid
+
+theorem thread1_valid : thread1.valid :=by
+  rw [Thread.valid]
+  apply valid_bind_mutex_lock
+
+  intro x0
   apply valid_bind (spec :=spec) λ ⟨⟩ r' => r' = Lock.Locked ⟨x0 + 1, x0⟩
   . -- validate ++x
     apply valid_rm
@@ -121,37 +158,14 @@ theorem thread1_valid : thread1.valid' Mt.Lock.Unlocked :=by
   intro r ⟨⟩ r_def
   rw [r_def]; clear r_def r
   . -- validate mutex release
-    apply valid_rm
-    simp only [spec, Lock.add_unlocked]
-    intro env_r ⟨⟨x, y⟩, locked ⟩ ⟨⟩ initial_valid
-    exists Lock.Unlocked
-    injection initial_valid.elim_locked.right.left
-    rename_i x_def y_def
-    simp only [initial_valid.elim_locked]
-    rw [x_def.symm, y_def.symm] ; clear x_def y_def
-    exact ⟨validate.unlocked rfl, rfl⟩
+    apply valid_mutex_release
+    rfl
 
-theorem thread2_valid : thread2.valid' Mt.Lock.Unlocked :=by
-  rw [valid']
-  apply valid_bind (spec :=spec) λ ⟨⟩ r => r.is_locked_and_valid Data.valid
-  . -- verify mutex lock
-    apply valid_blocking_rmr
-    simp only [spec, Lock.add_unlocked]
-    intro env_r s is_unlocked initial_valid
-    exists Lock.Locked s.data
-
-    have is_unlocked :=of_decide_eq_true is_unlocked
-    have :=initial_valid.elim_unlocked is_unlocked
-    
-    simp only [spec, this, Lock.is_locked_and_valid, and_true]
-    exact validate.locked ..
+theorem thread2_valid : thread2.valid :=by
+  rw [Thread.valid]
+  apply valid_bind_mutex_lock
   
-  intro r ⟨⟩ is_locked_and_valid
-  cases r <;> try contradiction
-  rename_i data0
-  let ⟨x0, y0⟩ :=data0 ; clear data0
-  cases is_locked_and_valid
-  
+  intro x0
   apply valid_bind (spec :=spec) λ px r' => r' = Lock.Locked ⟨x0, x0⟩ ∧ px = x0
   . -- verify read of x; we should get x0
     apply valid_read
@@ -198,14 +212,7 @@ theorem thread2_valid : thread2.valid' Mt.Lock.Unlocked :=by
   intro r ⟨⟩ r_def
   rw [r_def]; clear r_def r
   . -- validate mutex release
-    apply valid_rm
-    simp only [spec, Lock.add_unlocked]
-    intro env_r ⟨⟨x, y⟩, locked⟩ ⟨⟩ initial_valid
-    exists Lock.Unlocked
-    injection initial_valid.elim_locked.right.left
-    rename_i x_def y_def
-    simp only [initial_valid.elim_locked]
-    rw [x_def.symm, y_def.symm] ; clear x_def y_def
-    exact ⟨validate.unlocked rfl, rfl⟩
+    apply valid_mutex_release
+    rfl
 
 end SampleMutex
